cleanup in HSL

examples/low-mitls-experiments/HSL.fst
@@ -29,7 +29,8 @@ type loc = LowStar.Modifies.loc
  * So, the record layer appends to the buffer after p1
  * At some point (in HSL.process), HSL decides that the contents between p0 and p1 is a valid message
  * And at that point, it moves p0 and p1
- * msgs is the list of all subsequences in the buffer that don't contain a 0ul
+ * 
+ * We also keep msgs: list of all subsequences in the buffer that don't contain a 0ul
  *)
 abstract noeq type hsl_state =
   | Mk_state: len:u32 ->
@@ -46,11 +47,14 @@ abstract let hsl_get_p0 (st:hsl_state) :reference u32 = st.p0
 abstract let hsl_get_p1 (st:hsl_state) :reference u32 = st.p1
 abstract let hsl_get_msgs (st:hsl_state) :reference (list (u32 * u32)) = st.msgs
 
+(*
+ * Helper to state pairwise disjointness of locations
+ *)
 [@"opaque_to_smt"]
 unfold private let loc_pairwise_disjoint (s:TSet.set loc) :Type0 =
   forall (l1 l2:loc). TSet.mem l1 s ==> TSet.mem l2 s ==> Mods.loc_disjoint l1 l2
 
-(* liveness and disjointness *)
+(* Liveness and disjointness *)
 [@"opaque_to_smt"]
 unfold private let liveness_and_disjointness (st:hsl_state) (h:mem) :Type0 =
   let len, buf, p0, p1, msgs = hsl_get_len st, hsl_get_buf st, hsl_get_p0 st, hsl_get_p1 st, hsl_get_msgs st in
@@ -63,49 +67,51 @@ unfold private let liveness_and_disjointness (st:hsl_state) (h:mem) :Type0 =
 
   Buffer.live h buf /\ contains h p0 /\ contains h p1 /\ contains h msgs /\  //liveness
   Buffer.len buf == len /\  //buffer length
-  sel h p0 <=^ len /\  //p0 and p1 invariants
-  sel h p1 <=^ len /\
-  sel h p0 <=^ sel h p1
+  sel h p1 <=^ len /\  //p1 is leq len
+  sel h p0 <=^ sel h p1  //p0 is leq p1
 
-(* an invariant on the sequence content between p0 and p1 in the buffer *)
+(*
+ * An invariant on the sequence content between p0 and p1 in the buffer, that it doesn't contains 0ul
+ *
+ *)
 [@"opaque_to_smt"]
-unfold private let null_terminator_invariant_buf
-  (len:u32) (buf:Buffer.buffer u32) (p0 p1:u32)
-  (h:mem{Buffer.len buf == len /\ p1 <=^ len /\ p0 <=^ p1}) :GTot Type0
+unfold private let null_terminator_invariant_helper
+  (buf:Buffer.buffer u32) (p0:u32) (p1:u32{p1 <=^ Buffer.len buf /\ p0 <=^ p1}) (h:mem)
   = let subseq_size = p1 -^ p0 in
     let subseq = Buffer.as_seq h (Buffer.gsub buf p0 subseq_size) in
     forall (i:nat). i < v subseq_size ==> Seq.index subseq i =!= 0ul
 
+(* Lifted to hsl_state *)
 [@"opaque_to_smt"]
-unfold private let msgs_list_invariant_buf
-  (len:u32) (buf:Buffer.buffer u32) (l:list (u32 * u32)) (p0:u32{p0 <=^ len})
-  (h:mem{Buffer.len buf == len}) :GTot Type0
-  = forall (i j:u32). List.Tot.mem (i, j) l ==>
-                 (i <^ j /\ j <^ p0 /\
+unfold private let null_terminator_invariant (st:hsl_state) (h:mem{liveness_and_disjointness st h})
+  = let buf, p0, p1 = hsl_get_buf st, sel h (hsl_get_p0 st), sel h (hsl_get_p1 st) in
+    null_terminator_invariant_helper buf p0 p1 h
+
+(*
+ * An invariant on the list that all subsequences are 0ul free
+ *)
+[@"opaque_to_smt"]
+unfold private let msgs_list_invariant_helper
+  (buf:Buffer.buffer u32) (l:list (u32 * u32)) (p0:u32{p0 <=^ Buffer.len buf}) (h:mem)
+  = forall (i j:u32). List.Tot.mem (i, j) l ==>  //if (i, j) is in the list
+                 (i <^ j /\ j <^ p0 /\  //then both lie before p0
 		  (let subseq_size = j -^ i in
 		   let subseq = Buffer.as_seq h (Buffer.gsub buf i subseq_size) in
-		   forall (k:nat). k < v subseq_size ==> Seq.index subseq k =!= 0ul))
+		   forall (k:nat). k < v subseq_size ==> Seq.index subseq k =!= 0ul))  //and no 0ul
 
-(* an invariant on the sequence content between p0 and p1 in the buffer *)
+(* Lifted to hsl_state *)
 [@"opaque_to_smt"]
-unfold private let null_terminator_invariant (st:hsl_state) (h:mem{liveness_and_disjointness st h}) :GTot Type0 
-  = let buf, p0, p1 = hsl_get_buf st, sel h (hsl_get_p0 st), sel h (hsl_get_p1 st) in
-    null_terminator_invariant_buf (hsl_get_len st) buf p0 p1 h
+unfold private let msgs_list_invariant (st:hsl_state) (h:mem{liveness_and_disjointness st h})
+  = let buf, p0, msgs = hsl_get_buf st, sel h (hsl_get_p0 st), sel h (hsl_get_msgs st) in
+    msgs_list_invariant_helper buf msgs p0 h
 
-(* an invariant on the list of indices *)
+(* Combine the predicates above *)
 [@"opaque_to_smt"]
-unfold private let msgs_list_invariant (st:hsl_state) (h:mem{liveness_and_disjointness st h}) :GTot Type0 
-  = let len, buf, p0, msgs = hsl_get_len st, hsl_get_buf st, sel h (hsl_get_p0 st), sel h (hsl_get_msgs st) in
-    msgs_list_invariant_buf len buf msgs p0 h
+unfold private let hsl_invariant_predicate (st:hsl_state) (h:mem)
+  = liveness_and_disjointness st h /\ null_terminator_invariant st h /\ msgs_list_invariant st h
 
-[@"opaque_to_smt"]
-unfold private let hsl_invariant_predicate (st:hsl_state) (h:mem) :Type0 =
-  liveness_and_disjointness st h /\
-  null_terminator_invariant st h /\
-  msgs_list_invariant st h
-
-(* finally, the abstract invariant and its elimination *)
-abstract let hsl_invariant (st:hsl_state) (h:mem) :Type0 = hsl_invariant_predicate st h
+(* Finally, the abstract invariant and its elimination *)
+abstract let hsl_invariant (st:hsl_state) (h:mem) = hsl_invariant_predicate st h
 
 let lemma_hsl_invariant_elim (st:hsl_state) (h:mem)
   :Lemma (requires (hsl_invariant st h))
@@ -114,7 +120,7 @@ let lemma_hsl_invariant_elim (st:hsl_state) (h:mem)
   = ()
 
 (*
- * HSL footprint = p0, p1, and the buffer contents between p0 and p1 
+ * HSL footprint = p0, p1, buffer contents between p0 and p1, and msgs
  * This is not abstract, so that the client (Record) can append the buffer after p1, and use the framing lemma
  *)
 let hsl_footprint (st:hsl_state) (h:mem{hsl_invariant st h}) =
@@ -134,26 +140,16 @@ let lemma_frame_hsl_invariant (st:hsl_state) (l:loc) (h0 h1:mem)
 	 (ensures  (hsl_invariant st h1 /\ hsl_footprint st h1 == hsl_footprint st h0))
 	 [SMTPat (hsl_invariant st h0); SMTPat (loc_disjoint l (hsl_footprint st h0));
 	  SMTPat (Mods.modifies l h0 h1)]
-  = let buf, p0', p1, msgs = hsl_get_buf st, hsl_get_p0 st, hsl_get_p1 st, hsl_get_msgs st in
+  = let buf, p0, p1, msgs = hsl_get_buf st, hsl_get_p0 st, hsl_get_p1 st, hsl_get_msgs st in
 
     let b0 = Buffer.as_seq h0 buf in
     let b1 = Buffer.as_seq h0 buf in
-    let p0 = v (sel h0 p0') in
+    let p0 = v (sel h0 p0) in
     let p1 = v (sel h0 p1) in
 
-    let msgs0 = sel h0 msgs in
-    let msgs1 = sel h1 msgs in
-    assert (msgs0 == msgs1);
-
-    //we need this to prove the uncommented part below, essentially that the buffer
-    //contents did not change between p0 and p1
-    //we have buffer contents did not change from 0 to p1,
-    //it is a bit unfortunate that from that we can't SMT derive between p0 to p1
     assert (forall (k:nat). k < p1 ==> Seq.index b0 k == Seq.index (Seq.slice b0 0 p1) k);
     assert (forall (i j:nat) (k:nat). (i < j /\ j < p0 /\ k < (j - i)) ==>
                               Seq.index (Seq.slice b0 i j) k == Seq.index (Seq.slice b1 i j) k)
-    // assert (Seq.equal (Buffer.as_seq h0 (Buffer.gsub buf (sel h0 p0) (sel h0 p1 -^ sel h0 p0)))
-    //                   (Buffer.as_seq h1 (Buffer.gsub buf (sel h1 p0) (sel h1 p1 -^ sel h1 p0))))
 
 assume val fresh_loc: Mods.loc -> mem -> mem -> Type0
 
@@ -189,30 +185,34 @@ let hsl_create (len:u32{len >^ 0ul})
     st
 
 (*
- * Auxiliary function for processing the buffer, skip ahead
+ * Auxiliary function for processing the buffer
+ *
+ * Processes the buffer between p1 and p, one at a time
+ * Returns new p0, and updated list of indices
  *)
-private let rec aux_process (len:u32) (b:Buffer.buffer u32) (p0 p1 p:u32) (l:list (u32 * u32))
+private let rec aux_process (b:Buffer.buffer u32) (p0 p1 p:u32) (l:list (u32 * u32))
   :ST (u32 * list (u32 * u32))
       (requires (fun h0 -> Buffer.live h0 b /\
-                        len == Buffer.len b /\ p <=^ len /\ p1 <=^ p /\ p0 <=^ p1 /\
-                        null_terminator_invariant_buf len b p0 p1 h0 /\
-			msgs_list_invariant_buf len b l p0 h0))
+                        p <=^ Buffer.len b /\ p1 <=^ p /\ p0 <=^ p1 /\
+                        null_terminator_invariant_helper b p0 p1 h0 /\
+			msgs_list_invariant_helper b l p0 h0))
       (ensures  (fun h0 (r, l) h1 -> Buffer.live h1 b /\ 
 	                          r <=^ p /\
-				  null_terminator_invariant_buf len b r p h1 /\
-				  msgs_list_invariant_buf len b l r h1 /\
+				  null_terminator_invariant_helper b r p h1 /\
+				  msgs_list_invariant_helper b l r h1 /\
 	                          Mods.modifies loc_none h0 h1))
-  = if p = p1 then p0, l
+  = if p = p1 then p0, l  //done
     else
       let c = Buffer.index b p1 in
-      if c = 0ul then
-        if p0 = p1 then aux_process len b (p1 +^ 1ul) (p1 +^ 1ul) p l
-        else aux_process len b (p1 +^ 1ul) (p1 +^ 1ul) p ((p0, p1)::l)
-      else aux_process len b p0 (p1 +^ 1ul) p l
+      if c = 0ul then  //found a 0
+        if p0 = p1 then aux_process b (p1 +^ 1ul) (p1 +^ 1ul) p l  //if the subsequence is empty, just go ahead
+        else aux_process b (p1 +^ 1ul) (p1 +^ 1ul) p ((p0, p1)::l)  //else add it to the list
+      else aux_process b p0 (p1 +^ 1ul) p l
 
 (*
  * Main process function that client (Record) calls once it has appended some data to the input buffer
  * It updates the p0 and p1 pointers, so that p1 points to p (the input index)
+ * Also updates the msgs
  * And maintains the invariant
  *)
 let hsl_process (st:hsl_state) (p:u32)
@@ -224,7 +224,7 @@ let hsl_process (st:hsl_state) (p:u32)
 	                          Mods.modifies (Mods.loc_union (Mods.loc_mreference (hsl_get_p0 st))
 				                                (Mods.loc_mreference (hsl_get_p1 st))) h0 h1))
   = let len, buf, p0, p1, msgs = hsl_get_len st, hsl_get_buf st, hsl_get_p0 st, hsl_get_p1 st, hsl_get_msgs st in
-    let new_p0, new_msgs = aux_process len buf (!p0) (!p1) p (!msgs) in
+    let new_p0, new_msgs = aux_process buf !p0 !p1 p !msgs in
     p0 := new_p0;
     p1 := p;
     msgs := new_msgs
